Changing labeled language semantics for lang. equiv.

labeled/Semantics.v
@@ -1,48 +1,51 @@
-Require Export Syntax.
-Require Export Substitution.
+Require Import Syntax.
+Require Import Substitution.
 Require Import FSets.
+Require Import Arith.
 
-Open Scope is5_scope.
+Open Scope labeled_is5_scope.
 
 Global Reserved Notation " Omega ';' Gamma '|-' M ':::' A '@' w " (at level 70).
 
-Inductive types : worlds -> list (ty*wo) -> te -> ty -> var -> Prop :=
- | t_hyp: forall A w_n Gamma Omega v_n
+Definition Context_L := list (ty_L * wo).
+
+Inductive types_L : worlds_L -> Context_L -> te_L -> ty_L -> var -> Prop :=
+ | t_hyp_L: forall A w_n Gamma Omega v_n
    (Old: w_n \in Omega)
    (H_hyp: nth_error Gamma v_n = Some (A, fwo w_n)),
-     Omega; Gamma |- hyp v_n ::: A@w_n
- | t_lam: forall A A' w Gamma Omega M 
+     Omega; Gamma |- hyp_L v_n ::: A@w_n
+ | t_lam_L: forall A A' w Gamma Omega M 
    (H_lam: Omega; (A, fwo w)::Gamma |- M:::A'@w),
-     Omega; Gamma |- lam A M ::: A ---> A' @ w
- | t_appl: forall A A' w Gamma Omega M N
+     Omega; Gamma |- lam_L A M ::: A ---> A' @ w
+ | t_appl_L: forall A A' w Gamma Omega M N
    (H_appl1: Omega; Gamma |- N ::: A'@w)
    (H_appl2: Omega; Gamma |- M ::: A' ---> A @ w),
-     Omega; Gamma |- appl M N ::: A@w
- | t_box: forall L A w Gamma Omega M
+     Omega; Gamma |- appl_L M N ::: A@w
+ | t_box_L: forall L A w Gamma Omega M
    (Old: w \in Omega)
    (HT: forall w', w' \notin L -> \{w'} \u Omega; Gamma |- M^(fwo w')::: A @ w'),
-     Omega; Gamma |- box M ::: [*]A @  w
- | t_unbox: forall A w Gamma Omega M
+     Omega; Gamma |- box_L M ::: [*]A @  w
+ | t_unbox_L: forall A w Gamma Omega M
    (H_unbox: Omega; Gamma |- M ::: [*]A@w),
-     Omega; Gamma |- unbox M ::: A @ w
- | t_get: forall A w w' Gamma Omega M
+     Omega; Gamma |- unbox_L M ::: A @ w
+ | t_get_L: forall A w w' Gamma Omega M
    (New: w \in Omega) 
    (H_get: Omega; Gamma |- M ::: <*>A@w'),
-     Omega; Gamma |- get (fwo w') M ::: <*>A@w
- | t_letd: forall L A w B Gamma Omega M N
+     Omega; Gamma |- get_L (fwo w') M ::: <*>A@w
+ | t_letd_L: forall L A w B Gamma Omega M N
    (Old: w \in Omega)
    (H_letd: Omega; Gamma |- M ::: <*>A@w)
    (HT: forall w', w' \notin L -> 
      \{w'} \u Omega; (A, fwo w')::Gamma |- N^(fwo w'):::B@w),
-     Omega; Gamma |- letd M N ::: B@w
- | t_here: forall A w Gamma Omega M
+     Omega; Gamma |- letd_L M N ::: B@w
+ | t_here_L: forall A w Gamma Omega M
    (H_here: Omega; Gamma |- M ::: A@w),
-     Omega; Gamma |- here M ::: <*>A@w
- | t_fetch: forall A w w' Gamma Omega M
+     Omega; Gamma |- here_L M ::: <*>A@w
+ | t_fetch_L: forall A w w' Gamma Omega M
    (New: w \in Omega) 
    (H_fetch: Omega; Gamma |- M ::: [*]A@w'),
-     Omega; Gamma |- fetch (fwo w') M ::: [*]A@w
- where " Omega ';' Gamma '|-' M ':::' A '@' w " := (types Omega Gamma M A w) : is5_scope.
+     Omega; Gamma |- fetch_L (fwo w') M ::: [*]A@w
+ where " Omega ';' Gamma '|-' M ':::' A '@' w " := (types_L Omega Gamma M A w) : labeled_is5_scope.
 
 Fixpoint subst_typing Omega L D : Prop :=
 match L, D with
@@ -54,47 +57,47 @@ end.
 Global Reserved Notation " M |-> N " (at level 70).
 Global Reserved Notation " M |->* N " (at level 70).
 
-Inductive value: te -> Prop :=
-| val_lam: forall A M, value (lam A M)
-| val_box: forall M, value (box M)
-| val_here: forall M (HT: value M), value (here M)
+Inductive value_L: te_L -> Prop :=
+| val_L_lam: forall A M, value_L (lam_L A M)
+| val_L_box: forall M, value_L (box_L M)
+| val_L_here: forall M (HT: value_L M), value_L (here_L M)
 .
 
- Inductive step: te*wo -> te*wo -> Prop :=
- | red_appl_lam: forall A M N w,
+ Inductive step_LF: te_L*wo -> te_L*wo -> Prop :=
+ | red_appl_lam_L: forall A M N w,
    lc_w M -> lc_w N ->
-   (appl (lam A M) N, w) |-> ([N//0]M, w)
- | red_unbox_box: forall M w,
+   (appl_L (lam_L A M) N, w) |-> ([N//0]M, w)
+ | red_unbox_box_L: forall M w,
    lc_w_n M 1 ->
-   (unbox (box M), w) |-> (M^w, w)
- | red_letd_here: forall M N w (HVal: value M),
+   (unbox_L (box_L M), w) |-> (M^w, w)
+ | red_letd_here_L: forall M N w (HVal: value_L M),
    lc_w M -> lc_w_n N 1 ->
-   (letd (here M) N, w) |-> ([M//0](N^w), w)
- | red_appl: forall M N M' w (HRed: (M, w) |-> (M', w)),
+   (letd_L (here_L M) N, w) |-> ([M//0](N^w), w)
+ | red_appl_L: forall M N M' w (HRed: (M, w) |-> (M', w)),
    lc_w M -> lc_w N ->
-   (appl M N, w) |-> (appl M' N, w)
- | red_unbox: forall M M' w (HRed: (M, w) |-> (M', w)),
+   (appl_L M N, w) |-> (appl_L M' N, w)
+ | red_unbox_L: forall M M' w (HRed: (M, w) |-> (M', w)),
    lc_w M ->
-   (unbox M, w) |-> (unbox M', w)
- | red_fetch: forall M M' w w'  (HRed: (M, w) |-> (M', w)),
+   (unbox_L M, w) |-> (unbox_L M', w)
+ | red_fetch_L: forall M M' w w'  (HRed: (M, w) |-> (M', w)),
    lc_w M ->
-   (fetch w M, w') |-> (fetch w M', w')
- | red_fetch_val: forall w M w' (HVal: value M),
+   (fetch_L w M, w') |-> (fetch_L w M', w')
+ | red_fetch_val_L: forall w M w' (HVal: value_L M),
    lc_w M ->
-   (fetch w M, w') |-> ({w'//w}M, w')
- | red_here: forall N N' w (HRed: (N, w) |-> (N',w)),
+   (fetch_L w M, w') |-> ({w'//w}M, w')
+ | red_here_L: forall N N' w (HRed: (N, w) |-> (N',w)),
    lc_w N ->
-   (here N, w) |-> (here N', w)
- | red_letd: forall M M' N w (HRed: (M, w) |-> (M', w)),
+   (here_L N, w) |-> (here_L N', w)
+ | red_letd_L: forall M M' N w (HRed: (M, w) |-> (M', w)),
    lc_w M -> lc_w_n N 1 ->
-   (letd M N, w) |-> (letd M' N, w)
-| red_get: forall w M M' w' (HRed: (M, w) |-> (M', w)),
+   (letd_L M N, w) |-> (letd_L M' N, w)
+| red_get_L: forall w M M' w' (HRed: (M, w) |-> (M', w)),
    lc_w M ->
-   (get w M, w') |-> (get w M', w')
-| red_get_val: forall w M w' (HVal: value M),
+   (get_L w M, w') |-> (get_L w M', w')
+| red_get_val_L: forall w M w' (HVal: value_L M),
    lc_w M ->
-   (get w (here M), w') |-> (here {w'//w}M, w')
-where " M |-> N " := (step M N ) : is5_scope.
+   (get_L w (here_L M), w') |-> (here_L {w'//w}M, w')
+where " M |-> N " := (step_LF M N ) : labeled_is5_scope.
 
 
 Section Lemmas.
@@ -103,14 +106,11 @@ Lemma Weakening:
 forall Omega Gamma Delta M A w 
   (HT: Omega; Gamma |- M ::: A@w),
   Omega; Gamma ++ Delta |- M ::: A@w.
-intros; induction HT; eauto using types.
-  (* t_hyp *)
-  apply t_hyp. 
-    apply Old.
-    generalize dependent v_n.
-    induction Gamma; destruct v_n; intros; simpl in H_hyp; simpl; try discriminate.
-      apply H_hyp.
-      apply IHGamma; apply H_hyp.
+intros; induction HT; eauto using types_L.
+(* t_hyp *)
+constructor; [apply Old | generalize dependent v_n];
+induction Gamma; destruct v_n; intros; simpl in H_hyp; simpl; try discriminate;
+[ | apply IHGamma]; apply H_hyp.
 Qed.
 
 
@@ -118,23 +118,15 @@ Lemma WorldWeakening:
 forall Omega Gamma M A w w'
   (HT: Omega; Gamma |- M ::: A @ w),
   \{w'} \u Omega; Gamma |- M ::: A @ w.
-intros; induction HT; eauto using types.
-apply t_hyp.
-  rewrite in_union; right; assumption.
-  assumption.
-apply t_box with (L:=L).
+intros; induction HT; eauto using types_L;
+try (constructor; [rewrite in_union; right | ]; assumption).
+apply t_box_L with (L:=L).
   rewrite in_union; right; assumption.
   intros; rewrite union_comm_assoc; apply H; assumption.
-apply t_get.
-  rewrite in_union; right; assumption.
-  assumption.
-apply t_letd with (L:=L) (A:=A). 
+apply t_letd_L with (L:=L) (A:=A). 
   rewrite in_union; right; assumption.
   assumption.
   intros; rewrite union_comm_assoc; apply H; assumption.
-apply t_fetch.
-  rewrite in_union; right; assumption.
-  assumption.
 Qed.
 
 Lemma subst_t_type_preserv_end:
@@ -148,7 +140,7 @@ remember (Delta ++ (A, fwo w')::nil) as Delta';
 generalize dependent Delta;
 induction HT2;
 intros; simpl in *; subst; simpl;
-eauto using types.
+eauto using types_L.
 (* hyp *)
 destruct (eq_nat_dec (length Delta) v_n); subst.
 (* length Delta = v_n *)
@@ -165,7 +157,7 @@ induction Delta.
     replace Delta with (nil++Delta) by reflexivity;
     apply Weakening; assumption.
 (* length Delta <> v_n *)
-apply t_hyp; try assumption.
+apply t_hyp_L; try assumption.
 generalize dependent v_n;
 induction Delta; simpl in *; intros.
   (* nil *)
@@ -177,20 +169,20 @@ induction Delta; simpl in *; intros.
     simpl in *; assumption.
     simpl in *; apply IHDelta; auto.
 (* lam *)
-apply t_lam;
+apply t_lam_L;
 apply IHHT2;
 auto.
 (* box *)
-apply t_box with (L:=L); intros.
+apply t_box_L with (L:=L); intros.
 assumption.
 unfold open_w; rewrite subst_order_irrelevant.
 apply H.
   assumption.
-  apply WorldWeakening. assumption.
+  apply WorldWeakening; assumption.
   reflexivity.
   assumption.
 (* letd *)
-apply t_letd with (A:=A0)(L:=L); intros.
+apply t_letd_L with (A:=A0)(L:=L); intros.
 assumption.
 apply IHHT2; tauto.
 unfold open_w; rewrite subst_order_irrelevant.
@@ -223,9 +215,9 @@ auto.
 Qed.
 
 
-Fixpoint rename_world_context (w:wo) (w':wo) (Gamma: list (ty*wo)) : list(ty*wo):=
+Fixpoint rename_world_context (w:wo) (w':wo) (Gamma: Context_L) : Context_L:=
 match Gamma with
-| nil => @nil (ty*wo)
+| nil => @nil (ty_L*wo)
 | (A,w0) :: Gamma' => let w_res := if (eq_wo_dec w0 w') then w else w0 in
                       (A, w_res) :: rename_world_context w w' Gamma'
 end.
@@ -234,20 +226,15 @@ Lemma typing_renaming:
 forall Gamma n A w w'
   (HT: nth_error Gamma n = Some (A,w)),
   nth_error (rename_world_context w' w Gamma) n = Some (A, w').
-intros.
-generalize dependent n.
+intros;
+generalize dependent n;
 induction Gamma; intros.
 destruct n; simpl in *; discriminate.
-destruct a.
-simpl in *.
-induction n.
-simpl in *.
-inversion HT; subst.
-destruct (eq_wo_dec w w).
-  reflexivity.
-  elim n; reflexivity.
-simpl in *.
-apply IHGamma.
+destruct a; simpl in *; induction n; simpl in *.
+inversion HT; subst; 
+destruct (eq_wo_dec w w);
+[ | elim n]; reflexivity.
+apply IHGamma;
 assumption.
 Qed.
 
@@ -258,13 +245,12 @@ forall Gamma n A w w' w''
   nth_error (rename_world_context w' w Gamma) n = Some (A, w'').
 intros; generalize dependent n; induction Gamma; intros.  
 destruct n; simpl in *; discriminate.
-destruct a. 
-induction n; simpl in *;
-inversion HT.
+destruct a; induction n; 
+simpl in *; inversion HT.
   subst; destruct (eq_wo_dec w'' w).
     elim Neq; symmetry; assumption.
     reflexivity.
-  replace (nth_error Gamma n) with (Some (A, w'')). 
+  replace (nth_error Gamma n) with (Some (A, w''));
   apply IHGamma; assumption.
 Qed.
 
@@ -275,15 +261,14 @@ forall Omega Gamma M A w w' w'' w'''
   (HT: \{w} \u Omega; Gamma |- M ::: A @ w''),
   Omega; (rename_world_context (fwo w') (fwo w) Gamma) |- {fwo w'//fwo w}M ::: A @ w'''.
 intros; 
-remember (\{w} \u Omega) as Omega'.
+remember (\{w} \u Omega) as Omega';
 generalize dependent Omega;
 generalize dependent w''';
-generalize dependent w'.
-induction HT; intros.
+generalize dependent w';
+induction HT; intros; simpl.
 (* hyp *)
-simpl.
 destruct (eq_var_dec w_n w); subst;
-apply t_hyp.
+constructor.
 assumption.
 apply typing_renaming; assumption.
 rewrite in_union in Old; destruct Old.
@@ -294,56 +279,51 @@ apply typing_no_renaming.
   intro.
   inversion H; subst; elim n; reflexivity.
 (* lam *)
-simpl. apply t_lam.
+constructor;
 destruct (eq_var_dec w0 w); subst.
 (* w0 = w *)
-replace ((A, fwo w') :: rename_world_context (fwo w') (fwo w) Gamma) with (rename_world_context (fwo w') (fwo w) ((A, fwo w) :: Gamma)). 
+replace ((A, fwo w') :: rename_world_context (fwo w') (fwo w) Gamma) 
+   with (rename_world_context (fwo w') (fwo w) ((A, fwo w) :: Gamma)). 
 apply IHHT; auto.
 simpl; destruct (eq_wo_dec (fwo w) (fwo w)); [|elim n]; reflexivity.
 (* w0 <> w *)
-replace ((A, fwo w0) :: rename_world_context (fwo w') (fwo w) Gamma) with (rename_world_context (fwo w') (fwo w) ((A, fwo w0) :: Gamma)). 
+replace ((A, fwo w0) :: rename_world_context (fwo w') (fwo w) Gamma) 
+   with (rename_world_context (fwo w') (fwo w) ((A, fwo w0) :: Gamma)). 
 apply IHHT; auto.
-simpl. destruct (eq_wo_dec (fwo w0) (fwo w)).
+simpl; destruct (eq_wo_dec (fwo w0) (fwo w)).
   inversion e; elim n; assumption.
   reflexivity.  
 (* appl *)
-simpl; apply t_appl with (A':=A').
-apply IHHT1; assumption.
-apply IHHT2; assumption.
+apply t_appl_L with (A':=A');
+[apply IHHT1 | apply IHHT2]; assumption.
 (* box *)
-simpl; apply t_box with (L:=\{w} \u L).
+apply t_box_L with (L:=\{w} \u L).
 destruct (eq_var_dec w0 w); subst.
   assumption.
   rewrite in_union in Old; destruct Old.
-  apply notin_singleton in n; contradiction.
-  assumption.
-intros.
-apply notin_union_r in H0.
-destruct H0.
-unfold open_w in *.
-replace ({fwo w'0//bwo 0}({fwo w'//fwo w}M)) with ({fwo w'//fwo w}({fwo w'0//bwo 0}M)).
+    apply notin_singleton in n; contradiction.
+    assumption.
+intros; apply notin_union_r in H0;
+destruct H0; unfold open_w in *;
+replace ({fwo w'0//bwo 0}({fwo w'//fwo w}M)) 
+   with ({fwo w'//fwo w}({fwo w'0//bwo 0}M)).
 apply H.
-assumption.
-assert (w'0 <> w).
- intro. subst. elim H0. apply in_singleton_self.
-destruct (eq_var_dec w'0 w).
-  elim H2; assumption. 
-  reflexivity.
-rewrite in_union.
-right; assumption.
-subst. rewrite union_comm_assoc; reflexivity.
-apply subst_w_comm.
-intro.
-apply notin_singleton in H0.
+  assumption.
+  assert (w'0 <> w).
+    intro; subst; elim H0; apply in_singleton_self.
+  destruct (eq_var_dec w'0 w).
+    elim H2; assumption. 
+    reflexivity.
+  rewrite in_union; right; assumption.
+  subst; rewrite union_comm_assoc; reflexivity.
+apply subst_w_comm; intro;
+apply notin_singleton in H0;
 elim H0; symmetry; assumption.
 (* unbox *)
-simpl.
-apply t_unbox.
-apply IHHT; assumption.
+constructor; apply IHHT; assumption.
 (* get *)
-simpl.
 destruct (eq_wo_dec (fwo w') (fwo w));
-apply t_get;
+constructor
 destruct (eq_var_dec w0 w); subst;
 try assumption.
 rewrite in_union in New; destruct New.
@@ -379,7 +359,7 @@ apply IHHT.
     assumption.
 reflexivity.
 (* letd *)
-simpl. apply t_letd with (L:=\{w} \u L) (A:=A).
+apply t_letd_L with (L:=\{w} \u L) (A:=A).
 destruct (eq_var_dec w0 w); subst.
   assumption.
   rewrite in_union in Old.
@@ -412,14 +392,10 @@ apply IHHT.
   apply notin_singleton in H0.
   elim H0; reflexivity.
 (* here *)
-simpl.
-apply t_here.
-apply IHHT;
-assumption.
+constructor; apply IHHT; assumption.
 (* fetch *)
-simpl.
 destruct (eq_wo_dec (fwo w') (fwo w));
-apply t_fetch;
+constructor;
 destruct (eq_var_dec w0 w); subst;
 try assumption.
 rewrite in_union in New; destruct New.
@@ -461,8 +437,8 @@ Lemma Progress:
 forall Omega M A w 
   (H_lc: lc_w M)
   (HProgress: Omega; nil |- M ::: A@w),
-  value M \/ exists N, (M, fwo w) |-> (N, fwo w).
-induction M; intros; eauto using value; inversion HProgress; subst.
+  value_L M \/ exists N, (M, fwo w) |-> (N, fwo w).
+induction M; intros; eauto using value_L; inversion HProgress; subst.
 (* hyp *)
 destruct n; discriminate.
 (* appl *)
@@ -472,9 +448,9 @@ destruct (IHM1 (A'--->A) w  H1 H_appl2).
   (* value M1 *)
   inversion H; subst; inversion H_appl2; subst.
     inversion H1; subst;
-    eexists; apply red_appl_lam; auto.
+    eexists; apply red_appl_lam_L; auto.
   (* step *)
-  destruct H as [M1']; exists (appl M1' M2); apply red_appl; auto.
+  destruct H as [M1']; exists (appl_L M1' M2); apply red_appl_L; auto.
 (* unbox *)
 right;
 inversion H_lc; subst.
@@ -482,11 +458,11 @@ destruct (IHM ([*]A) w H0 H_unbox).
   (* value M *)
   inversion H; subst; inversion H_unbox; subst.
   exists (M0^(fwo w)).
-  apply red_unbox_box.
+  apply red_unbox_box_L.
   inversion H0; subst.
   assumption.
   (* step *)
-   destruct H as [M']; exists (unbox M'); apply red_unbox; auto.
+   destruct H as [M']; exists (unbox_L M'); apply red_unbox_L; auto.
 (* get *)
 right;
 inversion H_lc; subst.
@@ -494,9 +470,9 @@ destruct (IHM (<*>A0) w' H2 H_get).
   (* value M *)
   inversion H; subst; inversion H_get; subst.
     inversion H2; subst.
-    eexists; apply red_get_val; assumption.
+    eexists; apply red_get_val_L; assumption.
   (* step *)
-  destruct H as [M']; exists (get (fwo w') M'); apply red_get; auto.
+  destruct H as [M']; exists (get_L (fwo w') M'); apply red_get_L; auto.
 (* letd *)
 right;
 inversion H_lc; subst.
@@ -504,44 +480,47 @@ destruct (IHM1 (<*>A0) w H3 H_letd).
   (* value M1 *)
   inversion H; subst; inversion H_letd; subst.
   inversion H3; subst.
-  eexists; apply red_letd_here; assumption.
+  eexists; apply red_letd_here_L; assumption.
   (* step *)
-  destruct H as [M']; exists (letd M' M2); apply red_letd; auto.
+  destruct H as [M']; exists (letd_L M' M2); apply red_letd_L; auto.
 (* here *)
 inversion H_lc; subst.
 destruct (IHM A0 w H0 H_here).
   (* value *)
-  left; eauto using value.
+  left; eauto using value_L.
   (* step *)
-  right; destruct H as [M']; exists (here M'); apply red_here; auto.
+  right; destruct H as [M']; exists (here_L M'); apply red_here_L; auto.
 (* fetch *)
 right;
 inversion H_lc; subst.
 destruct (IHM ([*]A0) w' H2 H_fetch).
   (* value *)
   inversion H; subst; inversion H_fetch; subst.
-  eexists; apply red_fetch_val; assumption.
+  eexists; apply red_fetch_val_L; assumption.
   (* step *)
-  destruct H as [M']; exists (fetch (fwo w') M'); apply red_fetch; auto.
+  destruct H as [M']; exists (fetch_L (fwo w') M'); apply red_fetch_L; auto.
 Qed.
 
-(* TODO *)
-Axiom Fresh: forall (L:fset var), exists w0, w0 \notin L.
-
+Lemma Fresh: 
+  forall (L:fset var), exists w0, w0 \notin L.
+intro;
+exists (var_gen L);
+apply var_gen_spec.
+Qed.
 
 Lemma Preservation:
 forall Omega M N A w w' (HType: Omega; nil |- M ::: A@w) (HStep: (M, fwo w) |-> (N,fwo w')),
   Omega; nil |- N ::: A@w'.
 intros.
-remember (@nil (ty*wo)) as Gamma.
+remember (@nil (ty_L*wo)) as Gamma.
 generalize dependent N.
 generalize dependent w'.
 induction HType; intros;
 inversion HStep; subst;
-eauto using types.
+eauto using types_L.
 (* red_appl_lam *)
 inversion HType2; subst;
-replace ([N//0] M0) with (subst_list (N::nil) (length (@nil (te*wo))) M0) by auto;
+replace ([N//0] M0) with (subst_list (N::nil) (length (@nil (te_L*wo))) M0) by auto;
 apply subst_t_type_preserv with (Delta:=(A', fwo w')::nil).
   simpl; auto.
   simpl; assumption.
@@ -555,7 +534,7 @@ apply notin_union in H; destruct H.
 unfold open_w in *.
 replace ({fwo w'//bwo 0}M0) with ({fwo w'//bwo 0}({bwo 0//fwo x}({fwo x//bwo 0}M0))).
 rewrite subst_neutral.
-replace (@nil (ty*wo)) with (rename_world_context (fwo w') (fwo x) (@nil (ty*wo))).
+replace (@nil (ty_L*wo)) with (rename_world_context (fwo w') (fwo x) (@nil (ty_L*wo))).
 apply rename_w_type_preserv with (w'':=x).
 assumption.
 destruct (eq_var_dec x x). 
@@ -567,8 +546,8 @@ simpl; reflexivity.
 apply closed_step_opening; assumption.
 rewrite (subst_id M0 x 0 H1); reflexivity.
 (* red_get_here *)
-replace (here {fwo w'0//fwo w'}M0) with ({fwo w'0//fwo w'}(here M0)) by auto;
-replace (@nil (ty*wo)) with (rename_world_context (fwo w'0) (fwo w') nil) by auto.
+replace (here_L {fwo w'0//fwo w'}M0) with ({fwo w'0//fwo w'}(here_L M0)) by auto;
+replace (@nil (ty_L*wo)) with (rename_world_context (fwo w'0) (fwo w') nil) by auto.
 apply rename_w_type_preserv with (w'':=w').
   assumption.
   destruct (eq_var_dec w' w'). 
@@ -582,7 +561,7 @@ assert (exists w0, w0 \notin (L \u (free_worlds N))).
 apply Fresh.
 destruct H.
 apply notin_union in H; destruct H.
-replace ([M0//0](N^(fwo w'))) with (subst_list (M0::nil) (length (@nil (te*wo))) (N^(fwo w'))).
+replace ([M0//0](N^(fwo w'))) with (subst_list (M0::nil) (length (@nil (te_L*wo))) (N^(fwo w'))).
 apply subst_t_type_preserv with (Delta:=(A, fwo w')::nil).
   simpl; auto.
   simpl.
@@ -606,7 +585,7 @@ simpl; intros. destruct H1; subst.
   contradiction.
 simpl; reflexivity.
 (* red_fetch_val *)
-replace (@nil (ty*wo)) with (rename_world_context (fwo w'0) (fwo w') nil) by auto.
+replace (@nil (ty_L*wo)) with (rename_world_context (fwo w'0) (fwo w') nil) by auto.
 apply rename_w_type_preserv with (w'':=w').
   assumption.
   destruct (eq_var_dec w' w').
@@ -617,4 +596,4 @@ Qed.
 
 End Lemmas.
 
-Close Scope is5_scope.
+Close Scope labeled_is5_scope.
